monadproofs/proofs/reservebal.v
@@ -1,0 +1,5 @@
+(* proofs about reserve balances:
+- consensus guarnatees when it sends a block for executions
+- what consensus assumes execution guarantees
+- how those guarantees ensure execution will never run into a chase when an account has insufficient balance to pay gas fees
+ *)
